lecture14/simple-methods.dfy
@@ -1,0 +1,18 @@
+/* What *must* we assign to?  What *mustn't* we assign to? */
+method maxMethod(i : int, j : int) returns (mx : int, mn :int)
+{
+    if i < j { return j,i; }
+    return i,j;
+    // i := 3;
+}
+function max(i :int, j : int) : int
+{
+    if i< j then j
+    else i
+}
+method Main()
+{
+    // dafny is fussy here; can't put parens around x,n
+    var max1, min := maxMethod(10,10);
+    print "max is ", max, "min = ",min,"\n";
+}
