midsem/q1.dfy
@@ -1,0 +1,92 @@
+/* MID-SEMESTER EXAM 2026: Question 1.  
+
+   10 marks in total
+
+   All students to answer all questions. 
+
+   Replace /* YOUR WORK GOES HERE */ comments with your 
+   work.  Leave everything else untouched.
+
+   Remember that when asked to prove a lemma, you need to 
+   have a proof; sometimes {} will be enough, sometimes not,
+   but remember to always include the {}!
+
+*/
+
+datatype traffic_light = Red | Orange | Green
+
+/* 1A. 
+   Define the next_colour function with signature below so it 
+   returns the next colour after the input in the the standard
+   sequence of traffic light changes:
+      red -> green 
+      green -> orange
+      orange -> red
+
+   1 mark
+*/
+
+function next_colour(c : traffic_light) : traffic_light{
+   match c
+   case Red => Green
+   case Green => Orange
+   case Orange => Red
+}
+/* YOUR WORK GOES HERE */
+
+
+/* 1B. 
+   State and prove the lemma saying that 
+   Red's next colour is Green.
+   
+   1 mark
+*/
+lemma reds_next_colour()
+ensures next_colour(Red) == Green{}
+/* YOUR WORK GOES HERE */ 
+
+/* 1C. 
+   Define the n_step version of the above. This function takes 
+   n, a natural number, and c, a colour, and returns the result
+   of taking the next_colour n times. E.g., 
+     n_step(3, Red) == Red and n_step(2, Red) == Orange
+
+   2 marks
+*/
+function n_step(n : nat, c : traffic_light) : traffic_light
+{
+   if n == 0 then  c 
+   else n_step(n-1,next_colour(c))
+
+}
+/* YOUR WORK GOES HERE */
+
+/* 1D.
+   State and prove that the result of n_step(m+n,c) is 
+   the same as n_step(m, n_step(n, c))
+
+   2 marks
+*/
+lemma n_step_sum(m:nat, n : nat, c:traffic_light)
+ensures n_step(m+n,c) == n_step(m,n_step(n,c)){}
+/* YOUR WORK GOES HERE */
+
+/* 1E. 
+   State and prove that n_step(3,c) is always just c
+
+   1 mark
+*/
+lemma n_step3(c:traffic_light)
+ensures n_step(3,c) == c{}
+/* YOUR WORK GOES HERE */
+
+/* 1F. 
+   State and prove that n_step(3 * n, c) is always just c
+   You will need to use the n_step_sum result from above.
+
+   3 marks
+*/
+lemma n_step3n(n:nat, c:traffic_light)
+ensures n_step(3*n,c) == c
+
+/* YOUR WORK GOES HERE */
