midsem/q3.dfy
@@ -1,0 +1,105 @@
+/* MID-SEMESTER EXAM 2026: Question 3.  
+
+   10 marks in total
+
+   All students to answer all questions. 
+
+   Replace /* YOUR WORK GOES HERE */ comments with your 
+   work.  Leave everything else untouched.
+
+   Remember that when asked to prove a lemma, you need to 
+   have a proof.  Remember to include the {} and any 
+   necessary proof-steps within the braces !
+*/
+
+
+include "core-list.dfy"
+
+/* 3A.
+
+   Define the function that checks whether or not every 
+   element of a list of integers (an "ilist") is even 
+
+   1 mark.
+*/
+predicate listIsAllEven(l : ilist){
+   match l
+   case Nil => true
+   case Cons(x,xs) => if x%2 != 0 then false
+   else listIsAllEven(xs)
+}
+/* YOUR WORK GOES HERE */
+
+/* 3B. 
+ 
+   Prove the testing lemma stating that the list containing 
+   2 and 4, in that order, is all even.
+
+   1 mark
+*/
+lemma list24_isAllEven() 
+ensures listIsAllEven(Cons(2,Cons(4,Nil))){}
+/* YOUR WORK GOES HERE */
+
+/* 3C. 
+
+   Define the function that returns, in order, the 
+   list of all elements from the input list l that are 
+   even.
+
+   1 mark
+*/
+function filterEvens(l:ilist) : ilist{
+   match l
+   case Nil => Nil
+   case Cons(x,xs) => if x%2 == 0 then append(Cons(x,Nil),filterEvens(xs))
+   else filterEvens(xs)
+}
+/* YOUR WORK GOES HERE */
+
+/* 3D.
+
+   Prove the testing lemma that states that filterEvens on the 
+   list containing 2, 3, and 4, in that order returns the list
+   containing just 2 and 4, in that order.
+
+   1 mark
+*/
+lemma test_filterEvens234()
+ensures filterEvens(Cons(2,Cons(3,Cons(4,Nil)))) == Cons(2,Cons(4,Nil)) {}
+/* YOUR WORK GOES HERE */
+
+/* 3E.
+
+   State and prove the lemma that if a list is all evens, then
+   filterEvens on that list just returns the same list
+
+   2 marks
+*/
+lemma filterEvens_onAllEvensUnchanged(l:ilist)
+requires listIsAllEven(l)
+ensures l == filterEvens(l){}
+/* YOUR WORK GOES HERE */
+
+/* 3F.
+
+   State and prove the lemma that filterEvens on a list always
+   returns a list that has length less-than or equal to the length
+   of the input.
+
+   2 marks
+*/
+lemma length_filterEvens(l:ilist)
+ensures length(l) >= length(filterEvens(l)){}
+/* YOUR WORK GOES HERE */
+
+/* 3G.
+
+   State and prove the lemma that if a list is not all evens,
+   then filterEvens on that list returns a result that is shorter
+   than the input.  HINT: use the length_filterEvens result.
+
+   2 marks
+*/
+lemma filterEvens_onNotAllEvensShorter(l:ilist)
+/* YOUR WORK GOES HERE */
