midsem/q4.dfy
@@ -1,0 +1,97 @@
+/* MID-SEMESTER EXAM 2026: Question 4.  
+
+   10 marks in total
+
+   All students to answer all questions. 
+
+   Replace /* YOUR WORK GOES HERE */ comments with your 
+   work.  Leave everything else untouched.
+
+   Remember that when asked to prove a lemma, you need to 
+   have a proof.  Remember to include the {} and any 
+   necessary proof-steps within the braces !
+
+   The functions member and reverse from core-list.dfy
+   are particularly relevant in this question.
+*/
+
+include "core-list.dfy"
+
+
+/* 4A.
+
+   Define the function that returns the maximum element of a 
+   list of integers. Use a precondition to require that your 
+   function is not called on an empty list. You may use the 
+   max function below if desired.
+
+   2 marks
+*/
+function max(i:int, j:int) : int { if i < j then j else i }
+
+function maxList(l : ilist) : int{
+   match l
+   case Nil => 0
+   case Cons(x,xs) => max(x,maxList(xs))
+}
+/* YOUR WORK GOES HERE */
+
+/* 4B. 
+  
+   State and prove the testing lemma stating that maxList of the
+   value l123321, given below, is equal to 3
+
+   1 mark
+*/
+const l123321 := 
+  Cons(1, Cons(2, Cons(3, Cons(3, Cons(2, Cons(1,Nil))))))
+
+lemma maxList_l123321()
+ensures maxList(l123321) == 3{}
+/* YOUR WORK GOES HERE */
+
+/* 4C. 
+
+   State and prove that the max element of a non-empty list is a
+   member of that list
+
+   2 marks
+*/
+lemma maxList_member(l:ilist)
+requires length(l) > 0
+ensures member(maxList(l),l)
+
+/* YOUR WORK GOES HERE */
+
+/* 4D.
+
+   State and prove that if i is a member of an ilist, then it is
+   less-than or equal to the max value of that list
+
+   2 marks
+*/
+lemma maxList_maximal(i:int, l:ilist)
+requires member(i,l)
+ensures maxList(l) >= i{}
+/* YOUR WORK GOES HERE */
+
+/* 4E. 
+
+   State and prove that if l is a non-empty ilist, then the maximum
+   of the reverse of l is the maximum of the original list, l.
+
+   You will need to state, prove and use an auxiliary result along the 
+   way to get this result to come out.
+
+   3 marks
+*/
+
+lemma maxList_reverse(l:ilist)
+requires length(l) != 0
+ensures maxList(l) == maxList(reverse(l))
+{}
+//   case Cons(x,xs) => max(x,maxList(xs))
+//       case Cons(x,xs) => append(reverse(xs), Cons(x,Nil))
+
+
+/* YOUR WORK GOES HERE */
