midsem/q5.dfy
@@ -1,0 +1,109 @@
+/* MID-SEMESTER EXAM 2026: Question 5.  
+
+   10 marks in total
+
+   All students to answer all questions. 
+
+   Replace /* YOUR WORK GOES HERE */ comments with your 
+   work.  Leave everything else untouched (exception:
+   question 5E requires you to tweak an existing piece of 
+   text).
+
+   Remember that when asked to prove a lemma, you need to 
+   have a proof.  Remember to include the {} and any 
+   necessary proof-steps within the braces !
+
+   The functions take and drop from core-list.dfy
+   are particularly relevant in this question.
+*/
+
+include "core-list.dfy"
+
+/* 5A.
+
+   Define the function div3List which takes a list of 
+   integers and returns a new list where each element 
+   of the original has been divided by 3. (This is integer
+   division represented by the '/' operator.)
+   
+   1 mark
+*/
+
+function div3List(l : ilist) : ilist{
+   match l
+   case Nil => Nil
+   case Cons(x,xs) => Cons(x/3,div3List(xs))
+}
+/* YOUR WORK GOES HERE */
+
+/* 5B. 
+
+   State and prove the testing lemma stating that the
+   div3List function applied to elements 1 .. 6 returns
+   the list 0,0,1,1,1,2.
+
+   1 mark.
+*/
+const l123456 : ilist := 
+  Cons(1,Cons(2,Cons(3,Cons(4,Cons(5,Cons(6,Nil))))))
+lemma div3_123456()
+ensures div3List(l123456) == Cons(0,Cons(0,Cons(1,Cons(1,Cons(1,Cons(2,Nil)))))){}
+/* YOUR WORK GOES HERE */
+
+/* 5C.
+
+   State and prove the lemma stating that the length of 
+   div3List(l) is equal to the length of l.
+
+   1 mark.
+*/
+lemma length_div3List(l:ilist)
+ensures length(l) == length(div3List(l)){}
+/* YOUR WORK GOES HERE */
+
+/* 5D.
+
+   State and prove the lemma stating an integer i is a 
+   member of div3List(l) iff there exists a member of l 
+   which when divided by 3 is equal to i.
+
+   4 marks
+*/
+lemma member_div3(i:int, l : ilist)
+ensures exists x : int | member(x,l) :: member(x/3,div3List(l)) 
+
+/* YOUR WORK GOES HERE */
+
+/* 5E. 
+
+   Give the sumInThrees function below a termination argument
+   so that Dafny accepts it, proving any necessary lemmas 
+   along the way.  (take and drop come from core-list.dfy)
+
+   In other words: the definition of sumInThrees is broken 
+   because Dafny cannot prove that it terminates.
+   Write the necessary changes so it becomes something that 
+   Dafny accepts, while preserving the intended behaviour: 
+   test-cases for that intended behaviour include (using 
+   Haskell notation):
+     sumInThrees [1,2,3] == [6]
+     sumInThrees [1,2,3,4] == [6,4]
+     sumInThrees [] == [0]
+     sumInThrees [4,5,6,1,2,3,10] == [15,6,10]
+
+   There is no /* YOUR WORK GOES HERE */ tag in this question,
+   you should fix sumInThrees "in place".
+
+   3 marks
+*/    
+function sumInThrees(l:ilist) : ilist
+{
+    if length(l) <= 3 then Cons(sumList(l), Nil)
+    else Cons(sumList(take(3,l)), sumInThrees(drop(3,l)))
+}
+
+/* auxiliary used above */
+function sumList(l:ilist) : int
+{
+    match l case Nil => 0 case Cons(j,js) => j + sumList(js)
+}
