midsem/q6-COMP6260-only.dfy
@@ -1,0 +1,44 @@
+/* MID-SEMESTER EXAM 2026: Question 6.  
+
+   5 marks in total
+
+   This question is only for COMP6260 students. 
+
+   Replace /* YOUR WORK GOES HERE */ comments with your 
+   work.  Leave everything else untouched.
+
+   Remember that when asked to prove a lemma, you need to 
+   have a proof.  Remember to include the {} and any 
+   necessary proof-steps within the braces !
+
+*/
+
+ghost predicate divides(m:nat, n:nat)
+{
+    exists q : nat :: q * m == n
+}
+
+/* 6A. 
+
+   Prove that the divisibility relation, defined above is 
+   reflexive: i.e., any natural number n divides itself.
+
+   2 marks
+*/
+lemma divides_refl(n:nat)
+ensures divides(n,n)
+{
+   var n0 :| n0 * 1 == n0;
+}
+/* YOUR WORK GOES HERE */
+
+/* 6B.
+
+   Prove that the divisibility relation is transitive. 
+   In other words, if m divides n, and n divides p, then 
+   m also divides p.
+
+   3 marks
+*/
+lemma divides_trans(m:nat, n:nat, p:nat)
+/* YOUR WORK GOES HERE */
